README.md
@@ -1,2 +1,0 @@
-# T1-Metodos-Formais
-Trabalho 1 de Métodos Formais.
